\chapter{Svolgimento completo esercizio 5.7}

	\begin{align*}
		\sssssssvar & = (\lambda xyz.xz(yz))\ssssssvar\\
		& = (\lambda yz.\svar z(yz))\sssssvar\\
		& = (\lambda z.\svar z(\svar z))\ssssvar\\
		& = \ssvar(\ssvar)\sssvar\\
		& = (\lambda yz.\svar z(yz))(\ssvar)\sssvar\\
		& = (\lambda z.\svar z(\ssvar)z)\sssvar\\
		& = \ssvar(\sssvar)\ssvar\\
		& = (\lambda yz.\svar z(yz))(\sssvar)\ssvar\\
		& = (\lambda z.\svar z(\sssvar z))\ssvar\\
		& = \ssvar(\ssssvar)\svar\\
		& = (\lambda yz.\svar z(yz))(\ssssvar)\svar\\
		& = (\lambda z.\svar z(\ssssvar z))\svar\\
		& = \ssvar(\sssssvar)\\
		& = (\lambda yz.\svar z(yz))(\sssssvar)\\
		& = \lambda z.\svar z(\sssssvar z)\\
		& = \lambda z.(\lambda ya.a a(y a))(\sssssvar z)\\
		& = \lambda za.a a(\sssssvar a a)\\
		& = \lambda za.a a((\lambda yb.\svar b(y b))\sssvar z z)\\
		& = \lambda za.a a ((\lambda b.\svar b (\svar b)) \ssvar z z)\\
		& = \lambda za.a a (\ssvar (\ssvar) \svar a a)\\
		& = \lambda za.a a ((\lambda yb.\svar b (y b)) (\ssvar) \svar z z)\\
		& = \lambda za.a a ((\lambda b.\svar b (\ssvar b)) \svar z z)\\
		& = \lambda za.a a (\ssvar (\sssvar) a a)\\
		& = \lambda za.a a ((\lambda yb.\svar b (y b)) (\sssvar) z z)\\
		& = \lambda za.a a ((\lambda b.\svar b (\sssvar b)) z z)\\
		& = \lambda za.a a (\svar a (\sssvar a) a)\\
		& = \lambda za.a a ((\lambda yb.b b (y b)) (\sssvar z) z)\\
		& = \lambda za.a a ((\lambda b.b b (\sssvar b b)) z)\\
	\end{align*}
	\begin{align*}
		& = \lambda za.a a (a a (\sssvar a a))\\
		& = \lambda za.a a (a a ((\lambda yb.\svar b (y b)) \svar z z))\\
		& = \lambda za.a a (a a ((\lambda b.\svar b (\svar b)) z z))\\
		& = \lambda za.a a (a a (\svar a [\svar a] a))\\
		& = \lambda za.a a (a a ((\lambda yb.b b (y b)) (\svar z) z))\\
		& = \lambda za.a a (a a ((\lambda b.b b (\svar b b)) z))\\
		& = \lambda za.a a (a a (a a (\svar a a)))\\
		& = \lambda za.a a (a a (a a ((\lambda yb.b b (y b)) z)))\\
		& = \lambda za.a a (a a (a a (\lambda b.b b (b b))))\\
	\end{align*}
	